Core/Metatheory/FreeVars.lean
@@ -1,0 +1,90 @@
+import LeanSubst
+import Core.Typing
+
+open LeanSubst
+
+inductive Ty.FV : Ty -> Nat -> Prop where
+| var : FV t#x x
+| arrowr : FV a x -> FV (a -:> b) x
+| arrowl : FV b x -> FV (a -:> b) x
+| eqr : FV a x -> FV (a ~[K]~ b) x
+| eql : FV b x -> FV (a ~[K]~ b) x
+| appr : FV a x -> FV (a • b) x
+| appl : FV b x -> FV (a • b) x
+| all : FV p a -> FV (∀[K] p) (a + 1)
+
+
+instance instMembership_Nat_Ty : Membership Nat Ty where
+  mem := Ty.FV
+
+
+@[simp]
+def iterate (f : T -> T) : Nat -> T -> T
+| 0 => λ x => x
+| n + 1 => λ x => f $ (iterate f n) x
+
+notation f "^[" n "]" => iterate f n
+
+@[simp]
+theorem iterate_succ {x : Nat} : ((· + 1)^[n]) x = x + n := by
+  induction n <;> simp at *
+  case succ n ih => rw [ih]; omega
+
+
+theorem lift_iterated_succ_is_re :
+   ((Subst.lift (T := Ty))^[n]) +1 y = z ->
+   ∃ i, z = re i := by
+intro h
+induction n generalizing y z <;> simp at *
+case zero => exists y + 1; symm at h; assumption
+case succ n ih =>
+  cases y <;> simp at *
+  case zero => exists 0; symm at h; assumption
+  case succ y =>
+    simp [Subst.compose] at *
+    rcases ih with ⟨k, ih⟩
+    generalize zdef : (((Subst.lift (T := Ty))^[n]) +1) y = z at *
+    cases z <;> simp at *
+    case _ a => exists (a + 1); symm at h; assumption
+
+
+theorem FV.var_not_in_one_more {T : Ty} : (x ∉ T[((Subst.lift)^[x]) +1:Ty]) := by
+intro h
+induction T generalizing x <;> simp at *
+case var y =>
+  induction x generalizing y <;> simp at *
+  case zero => cases h
+  case succ n ih =>
+    simp [Subst.compose] at *
+    generalize zdef : (((Subst.lift (T := Ty))^[n]) +1 y) = z at *
+    cases z
+    case re z =>
+      replace ih := ih y
+      split at h <;> simp at *
+      case _ => cases h
+      case _ =>
+        rw[zdef] at ih; apply ih;
+
+        sorry
+    case su t =>
+      have lem := lift_iterated_succ_is_re zdef
+      rcases lem with ⟨_, lem⟩; cases lem
+case global => cases h
+case all P ih =>
+  replace ih := @ih (x + 1)
+  cases h <;> simp at *
+  case _ h => apply ih; sorry
+
+all_goals (
+case _ ih1 ih2 =>
+  replace ih1 := @ih1 x
+  replace ih2 := @ih2 x
+  cases h <;> simp at *
+  case _ h => apply ih1 h
+  case _ h => apply ih2 h)
+
+
+
+theorem FV.zero_not_in_succ {T : Ty} : 0 ∉ T[+1] := by
+have lem := @FV.var_not_in_one_more (T := T) 0
+simp at lem; apply lem
