Core/Ty/Substitution.lean
@@ -100,3 +100,55 @@ theorem Ty.apply_compose {s : Ty} {σ τ : Subst Ty} : s[σ][τ] = s[σ ∘ τ] 
 
 instance : SubstMapCompose Ty Ty where
   apply_compose := Ty.apply_compose
+
+theorem Ty.rename_preserves_var_shape {r : Ren} : t#x = T[r] -> ∃ y,  (T = t#y ∧ x = r y) := by
+intro h
+induction T <;> simp at *
+case var => simp [Ren.to] at h; assumption
+
+
+theorem Ty.rename_preserves_global_shape {r : Ren} : gt#x = T[r] -> T = gt#x := by
+intro h
+induction T <;> simp at *
+case var => simp [Ren.to] at h
+case global => symm at h; assumption
+
+
+theorem Ty.rename_preserves_arrow_shape {A B : Ty}{r : Ren} : A -:> B = T[r] ->
+  (∃ A' B' : Ty, (T = A' -:> B') ∧  A = A'[r] ∧ B = B'[r])
+:= by
+intro h
+induction T <;> simp at *
+case var => simp [Ren.to] at h
+case arrow a1 a2 _ _ => exists a1; exists a2
+
+theorem Ty.rename_preserves_eq_shape {A B : Ty}{r : Ren} : (A ~[K]~ B) = T[r] ->
+  (∃ A' B' : Ty, (T = A' ~[K]~ B') ∧  A = A'[r] ∧ B = B'[r])
+:= by
+intro h
+induction T generalizing K  <;> simp at *
+case var => simp [Ren.to] at h
+case eq a1 a2 _ _  =>
+  cases h.1; cases h.2.1; cases h.2.2; clear h
+  exists a1; exists a2
+
+theorem Ty.rename_preserves_app_shape {A B : Ty}{r : Ren} : (A • B) = T[r] ->
+  (∃ A' B' : Ty, (T = A' • B') ∧  A = A'[r] ∧ B = B'[r])
+:= by
+intro h
+induction T <;> simp at *
+case var => simp [Ren.to] at h
+case app a1 a2 _ _  =>
+  cases h.1; cases h.2; clear h
+  exists a1; exists a2
+
+
+theorem Ty.rename_preserves_all_shape {P : Ty}{r : Ren} : (∀[K] P) = T[r] ->
+  (∃ P' : Ty, (T = ∀[K]P') ∧  P = P'[re 0::↑r ∘ +1:Ty])
+:= by
+intro h
+induction T generalizing K P <;> simp at *
+case var => simp [Ren.to] at h
+case all a ih =>
+  cases h.1; cases h.2; clear h
+  exists a;
